src/frontends/lean/structure_cmd.cpp
@@ -1176,8 +1176,6 @@ struct structure_cmd_fn {
         name cases_on_name(m_name, "cases_on");
         add_rec_on_alias(cases_on_name);
         m_env = add_aux_recursor(m_env, cases_on_name);
-        if (is_inductive_predicate(m_env, m_name))
-            m_env = mk_drec(m_env, m_name);
     }
 
     // Return the parent names without namespace prefix
